src/db/subst_pres.lean
@@ -7,11 +7,20 @@ This file contains substitution preservation for `db` to `aeq`.
 import .injection
 import .subst
 
-theorem fin.succ_ne_zero {n : ℕ} : ∀ {N : fin n}, fin.succ N ≠ 0
-  | ⟨m, m_lt_n⟩ := fin.ne_of_vne (nat.succ_ne_zero m)
+namespace fin ------------------------------------------------------------------
 
-theorem fin.pred_succ {n : ℕ} : ∀ {N : fin n} {p : fin.succ N ≠ 0}, fin.pred (fin.succ N) p = N
+variables {n : ℕ}
+
+theorem succ_ne_zero : ∀ {N : fin n}, fin.succ N ≠ 0
+  | ⟨m, m_lt_n⟩ := ne_of_vne (nat.succ_ne_zero m)
+
+theorem pred_succ : ∀ {N : fin n} {p : fin.succ N ≠ 0}, pred (fin.succ N) p = N
   | ⟨m, m_lt_n⟩ p := rfl
+
+theorem succ_eq_add_right_1 : ∀ {N : fin n}, fin.succ N = add_right 1 N
+  | ⟨m, m_lt_n⟩ := rfl
+
+end /- namespace -/ fin --------------------------------------------------------
 
 namespace acie -----------------------------------------------------------------
 namespace db -------------------------------------------------------------------
@@ -22,13 +31,13 @@ variables {vs : Type → Type} [vset vs V] -- Type of variable name sets
 variables {X Y : vs V} -- Variable name sets
 variables {e : exp X} -- Expressions
 variables {m n : ℕ} -- De Bruijn indices
-variables {ϕX : ν∈ X → fin m} {ϕY : ν∈ Y → fin n} -- De Bruijn injections
+variables {ϕ ϕX : ν∈ X → fin m} {ϕY : ν∈ Y → fin n} -- De Bruijn injections
 variables {F : exp.subst X Y} -- Expression substitutions
 variables {G : db.subst m n} -- De Bruijn substitutions
 
 theorem injection_pres_subst.lam₁
 : (∀ (x : ν∈ X), inject (F x) ϕY = G (ϕX x))
-→ (∀ (x : ν∈ insert a X), inject (exp.subst.update a b F x) (inject.lam b ϕY) = subst.update G (inject.lam a ϕX x)) :=
+→ (∀ (x : ν∈ insert a X), inject (exp.subst.update a b F x) (inject.update b ϕY) = subst.update G (inject.update a ϕX x)) :=
   begin
     intros p x,
     cases x with x x_in_insert_a_X,
@@ -36,55 +45,138 @@ theorem injection_pres_subst.lam₁
     cases decidable.em (x = a),
     case or.inl : x_eq_a {
       simp [exp.subst.update],
-      conv {to_rhs, simp [inject.lam, subst.update]},
+      conv {to_rhs, simp [inject.update, subst.update]},
       repeat { rw dif_pos x_eq_a },
       rw dif_pos (@eq.refl (fin (nat.succ m)) 0),
-      simp [inject, vname.insert_self, inject.lam]
+      simp [inject, vname.insert_self, inject.update]
     },
     case or.inr : x_ne_a {
       simp [exp.subst.update],
-      conv {to_rhs, simp [inject.lam]},
+      conv {to_rhs, simp [inject.update]},
       repeat { rw dif_neg x_ne_a },
     }
 -/
     by_cases h : x = a,
     { /- h : x = a -/
       simp [exp.subst.update],
-      conv {to_rhs, simp [inject.lam, subst.update]},
+      conv {to_rhs, simp [inject.update, subst.update]},
       repeat {rw dif_pos h},
       rw dif_pos rfl,
-      simp [inject, vname.insert_self, inject.lam]
+      simp [inject, vname.insert_self, inject.update]
     },
     { /- h : x ≠ a -/
       simp [exp.subst.update],
-      conv {to_rhs, simp [inject.lam]},
+      conv {to_rhs, simp [inject.update]},
       repeat {rw dif_neg h},
       simp [subst.update],
       rw dif_neg fin.succ_ne_zero,
       rw fin.pred_succ,
+      generalize : vname.erase ⟨x, x_in_insert_a_X⟩ h = x',
+      rw ← p x',
+      generalize : F x' = e,
+/-
+      induction e,
+      case exp.var : Y y {
+/-
+        simp [exp.insert_var, exp.map, inject, shift_var, shift, vname.map_of_subset, inject.update, vname.erase, fin.shift],
+        rw if_neg (nat.not_lt_zero (ϕY y).val),
+        cases y with y y_in_Y,
+        by_cases h₂ : y = b,
+        { /- h₂ : y = b -/
+          rw dif_pos h₂,
+        },
+        { /- h₂ : y ≠ b -/
+        }
+-/
+      },
+-/
       admit
     }
   end
 
 theorem injection_pres_subst.lam₂
 : (∀ {X Y : vs V} {m n : ℕ} (F : exp.subst X Y) (G : db.subst m n) (ϕX : ν∈ X → fin m) (ϕY : ν∈ Y → fin n) (x : ν∈ X), inject (F x) ϕY = G (ϕX x))
-→ (∀ (x : ν∈ insert a X), inject (exp.subst.update a b F x) (inject.lam b ϕY) = subst.update G (inject.lam a ϕX x)) :=
+→ (∀ (x : ν∈ insert a X), inject (exp.subst.update a b F x) (inject.update b ϕY) = subst.update G (inject.update a ϕX x)) :=
   begin
     intros p x,
     cases x with x x_in_insert_a_X,
     cases decidable.em (x = a),
     case or.inl : x_eq_a {
       simp [exp.subst.update],
-      conv {to_rhs, simp [inject.lam, subst.update]},
+      conv {to_rhs, simp [inject.update, subst.update]},
       repeat { rw dif_pos x_eq_a },
       rw dif_pos (@eq.refl (fin (nat.succ m)) 0),
-      simp [inject, vname.insert_self, inject.lam]
+      simp [inject, vname.insert_self, inject.update]
     },
     case or.inr : x_ne_a {
       simp [exp.subst.update],
-      conv {to_rhs, simp [inject.lam]},
+      conv {to_rhs, simp [inject.update]},
       repeat { rw dif_neg x_ne_a },
-      exact p (exp.insert_var b ∘ F) (subst.update G) (fin.succ ∘ ϕX) (inject.lam b ϕY) (vname.erase ⟨x, x_in_insert_a_X⟩ x_ne_a)
+      exact p (exp.insert_var b ∘ F) (subst.update G) (fin.succ ∘ ϕX) (inject.update b ϕY) (vname.erase ⟨x, x_in_insert_a_X⟩ x_ne_a)
+    }
+  end
+
+theorem blah
+: inject (exp.insert_var (fresh X).1 e) (inject.update (fresh X).1 ϕ) = shift_var (inject e ϕ) :=
+  begin
+    induction e,
+    case exp.var : X x {
+      rw exp.insert_var.of_var x,
+      repeat {rw db.inject.var},
+      simp [shift_var],
+      -- rw db.shift.var 1 0 (ϕ x),
+      simp only [shift],
+      cases x with x x_in_X,
+      simp [vname.insert, inject.update],
+      cases fresh X with x' x'_not_in_X,
+      rw dif_neg (vname.ne_if_mem_and_not_mem ⟨x, x_in_X⟩ ⟨x', x'_not_in_X⟩),
+      simp [fin.shift],
+      rw if_neg (nat.not_lt_zero (ϕ ⟨x, x_in_X⟩).val),
+      simp [vname.erase],
+      rw ← fin.succ_eq_add_right_1,
+      refl
+    },
+    case exp.app : X f e rf re {
+      simp [shift_var],
+      rw inject.app,
+      -- rw shift.app m 1 0 (inject f ϕ) (inject e ϕ),
+      simp [shift],
+      rw exp.insert_var.of_app f e,
+      rw inject.app,
+      rw [rf, re],
+      refl
+    },
+    case exp.lam : X a e r {
+      rw inject.lam,
+      simp only [shift_var, shift],
+      rw exp.insert_var.of_lam₃ e,
+      rw inject.lam,
+    }
+  end
+
+theorem injection_pres_subst.lam₃
+: (∀ (x : ν∈ X), inject (F x) ϕY = G (ϕX x))
+→ ∀ (x : ν∈ insert a X), inject (exp.subst.update a (fresh Y).1 F x) (inject.update (fresh Y).1 ϕY) = subst.update G (inject.update a ϕX x) :=
+  begin
+    intros p x,
+    cases x with x x_in_insert_a_X,
+    -- cases fresh Y with y y_not_in_Y,
+    simp [exp.subst.update, db.inject.update],
+    by_cases h : x = a,
+    { /- h : x = a -/
+      repeat {rw dif_pos h},
+      rw inject.var,
+      simp [db.subst.update, db.inject.update]
+    },
+    { /- h₂ : x ≠ a -/
+      repeat {rw dif_neg h},
+      simp [db.subst.update],
+      rw dif_neg fin.succ_ne_zero,
+      rw fin.pred_succ,
+      generalize : vname.erase ⟨x, x_in_insert_a_X⟩ h = x',
+      rw ← p x',
+      generalize : F x' = e,
+     exact blah
     }
   end
 
@@ -106,10 +198,11 @@ theorem injection_pres_subst₁
     },
     case exp.lam : X a eX r {
       intro p,
-      conv {to_lhs, simp [exp.subst.apply, inject]},
-      conv {to_rhs, simp [inject, db.subst.apply]},
-      rw r (injection_pres_subst.lam₁ p),
-      refl
+      rw exp.subst.apply.of_lam eX,
+      rw db.inject.lam (exp.subst.apply _ _),
+      rw db.inject.lam eX,
+      rw db.subst.apply.lam (inject _ _),
+      rw r (injection_pres_subst.lam₃ p)
     }
   end
 
